move all list reasoning out of ZnWords,
and add it back as sparingly as possible where needed

bedrock2/src/bedrock2/ZnWordsTests.v
@@ -1,9 +1,100 @@
 Require Import Coq.ZArith.ZArith. Open Scope Z_scope.
 Require Import bedrock2.ZnWords.
 Require Import coqutil.Word.Interface.
+Require Import coqutil.Map.Interface.
+Require Import Coq.Lists.List. Import ListNotations.
+Require Import coqutil.Datatypes.Inhabited.
+Require Import bedrock2.Map.Separation.
+Require Import bedrock2.SepAutoArray bedrock2.SepAuto.
+Open Scope Z_scope.
+
+Local Hint Mode Word.Interface.word - : typeclass_instances.
+
+Infix "^+" := word.add  (at level 50, left associativity).
+Infix "^-" := word.sub  (at level 50, left associativity).
+Infix "^*" := word.mul  (at level 40, left associativity).
+Infix "^<<" := word.slu  (at level 37, left associativity).
+Infix "^>>" := word.sru  (at level 37, left associativity).
+Notation "/[ x ]" := (word.of_Z x)       (* squeeze a Z into a word (beat it with a / to make it smaller) *)
+  (format "/[ x ]").
+Notation "\[ x ]" := (word.unsigned x)   (* \ is the open (removed) lid of the modulo box imposed by words, *)
+  (format "\[ x ]").                     (* let a word fly into the large Z space *)
+Notation len := List.length.
+Coercion Z.of_nat : nat >-> Z.
+
+Fixpoint ands(Ps: list Prop): Prop :=
+  match Ps with
+  | P :: rest => P /\ ands rest
+  | nil => True
+  end.
 
 Section ZnWordTests.
-  Context {word: word.word 32} {word_ok: word.ok word}.
+  Context {word: word.word 32} {word_ok: word.ok word}
+          {mem: map.map word Init.Byte.byte} {mem_ok: map.ok mem}.
+
+  Goal forall (left0 right : word) (xs : list word),
+    word.unsigned (word.sub right left0) = 8 * Z.of_nat (Datatypes.length xs) ->
+    forall (x : list word) (x1 x2 : word),
+    word.unsigned (word.sub x2 x1) = 8 * Z.of_nat (Datatypes.length x) ->
+    word.unsigned (word.sub x2 x1) <> 0 ->
+    word.unsigned
+      (word.sub x2
+         (word.add
+            (word.add x1 (word.slu (word.sru (word.sub x2 x1) (word.of_Z 4)) (word.of_Z 3)))
+            (word.of_Z 8))) =
+    8 *
+    Z.of_nat
+      (Datatypes.length x -
+       S (Z.to_nat (word.unsigned (word.sub (word.add x1 (word.slu (word.sru (word.sub x2 x1)
+           (word.of_Z 4)) (word.of_Z 3))) x1) / word.unsigned (word.of_Z 8)))).
+  Proof.
+    intros. ZnWords.
+  Qed.
+
+  Let at_addr(addr: word)(clause: word -> mem -> Prop): mem -> Prop := clause addr.
+  Local Notation "addr |-> clause" := (at_addr addr clause)
+    (at level 25, format "addr  |->  '[' clause ']'").
+
+  Goal forall a : word,
+    let arguments := [a] in
+    forall (vs : list word) (R : mem -> Prop),
+    len vs = 3%nat ->
+    let w0 := List.nth 0 vs default in
+    let w1_0 := List.nth 1 vs default in
+    let w2_0 := List.nth 2 vs default in
+    let w1_1 := List.nth 0 vs default in
+    forall cond0 : bool,
+    let w2_1 := List.nth 0 vs default in
+    let w2_2 := if cond0 then w2_1 else w2_0 in
+    ands [~ \[w2_0] < \[w1_0]; ~ \[w0] < \[w1_0]] ->
+    let w1 := w1_1 in
+    let w2 := w2_0 in
+    ~ \[w2] < \[w1] ->
+    forall m : mem,
+    seps [a |-> word_array ([w1_0] ++ [w1] ++ List.skipn 2 vs); R] m ->
+    (forall (vs0 vs1 : list word) (v : word) (vs2 : list word),
+     vs0 = vs1 ++ [v] ++ vs2 /\ len vs1 = Z.to_nat (\[a ^+ /[8] ^- a] / 4) ->
+     Lift1Prop.iff1
+       (sep (a |-> word_array vs1)
+          (sep ((a ^+ /[8]) |-> scalar v)
+             ((a ^+ /[4 * S (Z.to_nat (\[a ^+ /[8] ^- a] / 4))]) |-> word_array vs2)))
+       (a |-> word_array vs0)) ->
+    forall m' : mem,
+    sep ((a ^+ /[8]) |-> scalar w2)
+      (sep R
+         (sep
+            (a |-> word_array
+                     (List.firstn (Z.to_nat (\[a ^+ /[8] ^- a] / 4))
+                        ([w1_0] ++ [w1] ++ List.skipn 2 vs)))
+            ((a ^+ /[4 * S (Z.to_nat (\[a ^+ /[8] ^- a] / 4))]) |->
+             word_array
+               (List.skipn (S (Z.to_nat (\[a ^+ /[8] ^- a] / 4)))
+                  ([w1_0] ++ [w1] ++ List.skipn 2 vs))))) m' ->
+    len (List.firstn (Z.to_nat (\[a ^+ /[8] ^- a] / 4)) ([w1_0] ++ [w1] ++ List.skipn 2 vs)) =
+    Z.to_nat (\[a ^+ /[8] ^- a] / 4).
+  Proof.
+    intros. list_length_rewrites_without_sideconds_in_goal. ZnWords.
+  Qed.
 
   Goal forall (a a' SZ: word) (T: Type) (f: T -> nat) (vs1: T),
       word.unsigned (word.sub a' a) mod word.unsigned SZ = 0 ->
@@ -18,7 +109,6 @@ Section ZnWordTests.
        TODO remove the rewrite if lia is fixed. *)
     rewrite H0.
     ZnWords.
-    all: fail "remaining subgoals".
-  Abort.
+  Qed.
 
 End ZnWordTests.
